
Comma Category Characterization of an
Adjunction

Definition 1 (Comma Category). We define the comma category F ↓ G of two functors
F : C → E and G : D → E as follows. Its objects are triples (A,B, f), where A is an
object in C, B is an object in D, and f : F (A)→ G(B) is an arrow in E. Furthermore,
an arrow (i, j) : (A,B, f) → (A′, B′, g) in F ↓ G is a pair of arrows i : A → A′ and
j : B → B′, such that the following diagram commutes:

FA GB

FA′ GB′

f

F i Gj

g

Theorem 1. Let F : D � C : G be two functors and ϕ : F ↓ IdC � IdD ↓ G : ψ an
isomorphism that is the identity on arrows then F a G.

Proof. We define the adjunction F a G by an isomorphism between the hom-sets
HomC(FA,B) and HomD(A,GB) that is natural in A and B. We define both sides
of the isomorphism ϕ′ : HomC(FA,B) � HomD(A,GB) : ψ′ by ϕ′(f) = π3(ϕ(A,B, f))
and ψ′(g) = π3(ψ(A,B, g)), where π3 extracts the arrow f from an object (A,B, f) in
the comma category.

• ϕ′ and ψ′ are an isomorphism, i.e., ψ′◦ϕ′ = id and ϕ′◦ψ′ = id . For all f : FA→ B
and g : A→ GB, it follows

ψ′(ϕ′(f)) = ψ′(π3(ϕ(A,B, f))) ϕ′(ψ′(g)) = ϕ′π3(ψ(A,B, f)))

= π3(ψ(A,B, π3(ϕ(A,B, f))) = π3(ϕ(A,B, π3(ψ(A,B, g)))

= π3(ψ(ϕ(A,B, f))) = π3(ϕ(ψ(A,B, g)))

= π3(A,B, f) = π3(A,B, g)

= f = g.

• ϕ′ is natural in A,B, i.e., for all i : A → A′, j : B → B′, and f : FA → B,
ϕ′(j ◦ f ◦ Fi) = Gj ◦ ϕ′(f) ◦ i as in the following commuting diagram

1



HomC(FA,B) HomD(A,GB)

HomC(FA′, B′) HomD(A′, GB′).

ϕ′

j ◦ − ◦ Fi Gj ◦ − ◦ i

ϕ′

First, observe how ϕ acts on arrows. An arrow (i, j) : (A,B, f) → (A′, B′, g) in
F ↓ IdC is mapped to an arrow (i, j) : (A,B,ϕ′(f)) → (A′, B′, ϕ′(g)) in IdD ↓ G.
This means, for a commuting square in the C, we obtain a commuting square in
D:

FA B A GB

FA′ B′ A′ GB′

f

F i j

ϕ′(f)

i Gj

g ϕ′(g)

In other words, we can use ϕ to do basic rewrite steps on ϕ′ if we provide a suitable
commuting squares in C.

With this technique, we prove the naturality of ϕ′ with three rewrite steps and
functoriality of G:

ϕ′(j ◦ f ◦ Fi) I
= ϕ′(j ◦ f) ◦ i
II
= G(j ◦ f) ◦ ϕ′(Fi)
= Gj ◦Gf ◦ ϕ′(Fi)
III
= Gj ◦ ϕ′(f) ◦ i

I ϕ′(j ◦ f ◦ Fi) = ϕ′(j ◦ f) ◦ i

(A,B′, j ◦ f ◦ Fi) (A,B′, ϕ′(j ◦ f ◦ Fi))

(A′, B′, j ◦ f) (A′, B′, ϕ′(j ◦ f))

(i,id) (i,id)
ϕ

FA B′ A GB′

FA′ B′ A′ GB′

j◦f◦Fi

F i id

ϕ′(j◦f◦Fi)

i G(id)

j◦f ϕ′(j◦f)

II ϕ′(j ◦ f) ◦ i = G(j ◦ f) ◦ ϕ′(Fi)
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(A,FA′, F i) (A,FA′, ϕ′(Fi))

(A′, B′, j ◦ f) (A,B′, ϕ′(j ◦ f))

(i,j◦f) (i,j◦f)
ϕ

FA FA′ A GFA′

FA′ B′ A′ GB′

Fi

F i j◦f

ϕ′(Fi)

i G(j◦f)
j◦f ϕ′(j◦f)

III Gf ◦ ϕ′(i) = ϕ′f ◦ i

(A,FA′, F i) (A,FA′, ϕ′(Fi))

(A′, B′, f) (A,B′, ϕ′(f))

(i,f) (i,f)
ϕ

FA FA′ A GFA′

FA′ B′ A′ GB′

Fi

F i f

ϕ′(Fi)

i Gf

f ϕ′(f)

• ψ′ natural in A,B is analogous to naturality of ϕ′.
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